@prefix : <http://lari-datasets.ilc.cnr.it/lemonEty#> .
@prefix dct: <http://purl.org/dc/terms/> .
@prefix lexinfo: <http://www.lexinfo.net/ontology/2.0/lexinfo#> .
@prefix ontolex: <http://www.w3.org/ns/lemon/ontolex#> .
@prefix owl: <http://www.w3.org/2002/07/owl#> .
@prefix rdf: <http://www.w3.org/1999/02/22-rdf-syntax-ns#> .
@prefix rdfs: <http://www.w3.org/2000/01/rdf-schema#> .
@prefix xml: <http://www.w3.org/XML/1998/namespace> .
@prefix xsd: <http://www.w3.org/2001/XMLSchema#> .

:Cognate a rdfs:Class ;
    rdfs:label "Cognate"@en ;
    rdfs:comment "'Cognate' is a subclass of Lexical Entry that consists of lexemes which are cognates of another Lexical Entry."@en ;
    rdfs:subClassOf ontolex:LexicalEntry .

:EtyLink a rdfs:Class ;
    rdfs:label "Etymological Link"@en ;
    rdfs:comment "'Etymological Link' is a class that consists of individuals that represent the etymological relationship between two linguistic entities."@en .

:Etymology a rdfs:Class ;
    rdfs:label "Etymology"@en ;
    rdfs:comment "'Etymology' is a class that consists of individuals that describe the history of a Lexical Entry."@en .

:Etymon a rdfs:Class ;
    rdfs:label "Etymon"@en ;
    rdfs:comment "'Etymon' is a subclass of Lexical Entry that consists of invidividuals whose role is to describe the origin and history of another Lexical Entry."@en ;
    rdfs:subClassOf ontolex:LexicalEntry .

<http://lari-datasets.ilc.cnr.it/lemonEty#> a owl:Ontology ;
    dct:contributor <http://www.ilc.cnr.it/en/content/anas_fahad_khan> ;
    dct:description "lemonEty is an extension of the ontolex-lemon model that provides concepts and properties that are useful in representing etymological information."@en ;
    dct:issued "2018-05-04" ;
    dct:rights "CC-BY" ;
    dct:title "lemonEty"@en ;
    owl:imports <http://www.w3.org/ns/lemon/all>,
        <http://www.w3.org/ns/lemon/ontolex> ;
    owl:versionInfo "Version 0.1.0" .

:cognate a rdf:Property,
        owl:ObjectProperty ;
    rdfs:label "cognate"@en ;
    rdfs:comment "'cognate' is an object property linking a linguistic entity with a Cognate."@en ;
    rdfs:range :Cognate .

:etyLinkType a rdf:Property,
        owl:DatatypeProperty ;
    rdfs:label "etymological link type"@en ;
    rdfs:comment "'etymological link type' specifies the type of a Etymological Link."@en ;
    rdfs:range :EtyLink .

:etySource a rdf:Property,
        owl:ObjectProperty ;
    rdfs:label "etymological source"@en ;
    rdfs:comment "'etymological source' is an object property that links an EtyLink with a linguistic entity which is the source of the relationship which the former represents."@en ;
    rdfs:domain :EtyLink .

:etySubSource a rdf:Property,
        owl:ObjectProperty ;
    rdfs:label "etymological sub-source"@en ;
    rdfs:comment "'etymological sub-source' is an object property that further specifies the etymological source of an EtyLink (assuming a prior use of etySource)."@en ;
    rdfs:domain :EtyLink .

:etySubTarget a rdf:Property,
        owl:ObjectProperty ;
    rdfs:label "etymological sub-target"@en ;
    rdfs:comment "'etymological sub-target' is an object property that further specifies the etymological target of an EtyLink (assuming a prior use of etyTarget)."@en ;
    rdfs:domain :EtyLink .

:etyTarget a rdf:Property,
        owl:ObjectProperty ;
    rdfs:label "etymological target"@en ;
    rdfs:comment "'etymological target' is an object property that links an EtyLink with a linguistic entity which is the target of the relationship which the former represents."@en ;
    rdfs:domain :EtyLink .

:etymology a rdf:Property,
        owl:ObjectProperty ;
    rdfs:label "etymology"@en ;
    rdfs:comment "'etymology' is  an object property linking a linguistic entity with an Etymology."@en ;
    rdfs:range :Etymology .

:etymon a rdf:Property,
        owl:ObjectProperty ;
    rdfs:label "etymon"@en ;
    rdfs:comment "'etymon' is  an object property that relates an Etymology with its related etymons."@en ;
    rdfs:domain :Etymology ;
    rdfs:range :Etymon .

:isCognateOf a rdf:Property,
        owl:ObjectProperty ;
    rdfs:label "isCognateOf"@en ;
    rdfs:comment "'is cognate of' is an object property linking a Cognate with some linguistic entity."@en ;
    rdfs:domain :Cognate .

:isEtyLinkOf a rdf:Property,
        owl:ObjectProperty ;
    rdfs:label "is etymological link of"@en ;
    rdfs:comment "'is etymological link of' is an object property that relates an Etymology with an Etymological Link."@en ;
    rdfs:domain :EtyLink ;
    rdfs:range :Etymology .

:isEtymologyOf a rdf:Property,
        owl:ObjectProperty ;
    rdfs:label "is etymology of"@en ;
    rdfs:comment "'is etymology of' is an object property linking an Etymology with a linguistic entity."@en ;
    rdfs:domain :Etymology .

:isEtymonOf a rdf:Property,
        owl:ObjectProperty ;
    rdfs:label "is etymon of"@en ;
    rdfs:comment "'is etymon of' is an object property that relates an Etymon with the etymologies it is a part of."@en ;
    rdfs:domain :Etymon ;
    rdfs:range :Etymology .

:startingLink a rdf:Property,
        owl:ObjectProperty ;
    rdfs:label "starting link"@en ;
    rdfs:comment "'starting link' is  an object property that relates an Etymology with its first Etymological Link."@en ;
    rdfs:domain :Etymology ;
    rdfs:range :EtyLink ;
    rdfs:subPropertyOf :hasEtyLink .

:hasEtyLink a rdf:Property,
        owl:ObjectProperty ;
    rdfs:label "has etymological link"@en ;
    rdfs:comment "'has etymological link' is an object property that relates an Etymology with one of its constituent Etymological Link objects."@en ;
    rdfs:domain :Etymology ;
    rdfs:range :EtyLink .

